Drop the record

state/SharedRefs.fst
@@ -8,13 +8,25 @@ let secret_map : map_sharedT = (** In Pulse, this can be a ghost reference and `
 (** Popular vote for this, instead of the top-level effectful call **)
 assume val secret_map : map_sharedT
 
-private
+let map_shared = FStar.Ghost.hide secret_map (** CA: this is also effectful **)
+
 let is_shared : ref_heap_stable_pred = (fun #a #p (r:mref a p) h ->
     h `contains` secret_map /\ (** this contains is necessary to show that is_shared is a stable predicate **)
     (sel h secret_map) (addr_of r)) 
 
-private
-let unmodified_map_implies_same_shared_status (ms:Set.set nat) (h0 h1:heap) : 
+let share = (fun #a #p sr -> 
+    let h0 = get () in
+    lemma_next_addr_contained_refs_addr h0 sr;
+    let m = !secret_map in
+    let m' = (fun p -> if p = addr_of sr then true else m p) in
+    secret_map := m';
+    let h1 = get () in
+    lemma_next_addr_upd_tot h0 secret_map m'
+  )
+
+let lemma_fresh_ref_not_shared = (fun #a #rel r h -> ())
+
+let lemma_unmodified_map_implies_same_shared_status (ms:Set.set nat) (h0 h1:heap) : 
     Lemma (h0 `contains` secret_map /\ h0 `heap_rel` h1 /\ ~(addr_of secret_map `Set.mem` ms) /\ modifies ms h0 h1 ==> 
       (forall #a #rel (r:mref a rel). is_shared r h0 <==> is_shared r h1)) = 
     introduce h0 `contains` secret_map /\ h0 `heap_rel` h1 /\ ~(addr_of secret_map `Set.mem` ms) /\ modifies ms h0 h1 ==> (forall #a #rel (r:mref a rel). is_shared r h0 <==> is_shared r h1) with _. begin
@@ -24,155 +36,4 @@ let unmodified_map_implies_same_shared_status (ms:Set.set nat) (h0 h1:heap) :
       end
     end  
 
-let shareS : sigT = {
-  map_shared = secret_map;
-  is_shared = is_shared;
-  fresh_ref_not_shared = (fun #a #rel r h -> ());
-  unmodified_map_implies_same_shared_status = unmodified_map_implies_same_shared_status;
-  same_addr_same_sharing_status = (fun ra rb h -> ());
-  share = (fun #a #p sr -> 
-    let h0 = get () in
-    lemma_next_addr_contained_refs_addr h0 sr;
-    let m = !secret_map in
-    let m' = (fun p -> if p = addr_of sr then true else m p) in
-    secret_map := m';
-    let h1 = get () in
-    lemma_next_addr_upd_tot h0 secret_map m'
-  );
-}
-
-  (**
-val is_shared_stable : #a:Type0 -> r:ref a -> Lemma (stable (shareS.is_shared r)) [SMTPat (shareS.is_shared r)]
-let is_shared_stable #a r : Lemma (stable (shareS.is_shared r)) [SMTPat (shareS.is_shared r)] = ()
-  (**assert (stable (shareS.is_shared r)) by (
-    norm[delta_only [`%stable;`%heap_rel];iota];
-    let h1 = forall_intro () in let h2 = forall_intro () in
-    let i = implies_intro () in 
-    let (x, y) = destruct_and i in
-    clear i;
-    let y = instantiate y (fresh_uvar None) in
-    let y' = instantiate y (fresh_uvar None) in
-    let y'' = instantiate y' (`secret_map) in
-    clear y; clear y';
-    compute ();
-    binder_retype (nth_binder 6); compute (); trefl ();
-    dump "H"
-  )**)
-
-val progr_sep_test: 
-  #rp: ref int -> 
-  ctx:(unit -> ST unit (fun _ -> True) (fun h0 _ h1 -> modifies_only_shared h0 h1)) ->
-  ST unit
-    (requires (fun h0 -> 
-      h0 `contains` rp /\
-      ~(shareS.is_shared rp h0)))
-    (ensures (fun h0 _ h1 ->
-      sel h0 rp == sel h1 rp)) // the content of rp should stay the same before/ after calling the context
-
-let progr_sep_test #rp f = 
-  f ()
-
-val progr_declassify :
-  rp: ref int -> 
-  ctx:(r:(ref int) -> IST unit (fun h0 -> h0 `contains` r /\ shareS.is_shared r h0) (ensures (fun h0 _ h1 -> modifies_only_shared h0 h1))) ->
-  IST unit
-    (requires (fun h0 -> 
-      h0 `contains` rp /\
-      ~(shareS.is_shared rp h0)))
-    (ensures (fun h0 _ h1 -> True))
-let progr_declassify rp f =
-  shareS.share rp;
-  f rp
-
-val progr_declassify_nested:
-  rp: ref (ref int) -> 
-  ctx:(r:(ref (ref int)) -> IST unit 
-    (requires (fun h0 -> h0 `contains` r /\ h0 `contains` (sel h0 r) /\ shareS.is_shared r h0 /\ shareS.is_shared (sel h0 r) h0))
-    (ensures (fun h0 _ h1 -> modifies_only_shared h0 h1))) ->
-  IST unit
-    (requires (fun h0 -> 
-      h0 `contains` rp /\ h0 `contains` (sel h0 rp) /\
-      ~(shareS.is_shared rp h0)))
-    (ensures (fun h0 _ h1 -> True))
-let progr_declassify_nested rp f =
-  shareS.share rp;
-  let p = !rp in
-  shareS.share p;
-  f rp
-
-val progr_secret_unchanged_test: 
-  rp: ref int -> 
-  rs: ref (ref int) ->
-  ctx:(unit -> IST unit (fun _ -> True) (fun h0 _ h1 -> modifies_only_shared h0 h1)) ->
-  IST unit 
-    (requires (fun h0 -> 
-      h0 `contains` rp /\ h0 `contains` rs /\ h0 `contains` (sel h0 rs) /\
-      ~(shareS.is_shared rp h0) /\
-      rp =!= (sel h0 rs) /\
-      shareS.is_shared rs h0 /\ shareS.is_shared (sel h0 rs) h0))
-    (ensures (fun h0 _ h1 ->
-      sel h0 rp == sel h1 rp))
-         
-let progr_secret_unchanged_test rp rs ctx = 
-  let h0 = get () in
-  let secret: ref int = alloc 0 in
-  assume (addr_of secret == next_addr h0);(** has to come from alloc, necessary to show that secret is not shared **)
-  let h1 = get () in
-  assume (next_addr h0 < next_addr h1); (** comes from alloc **)
-  ctx ();
-  let v = !secret in
-  assert (v == 0);
-  ()
-
-val progr_passing_callback_test: 
-  rp: ref int -> 
-  rs: ref (ref int) ->
-  //ctx:(elab_typ (TArr (TArr TUnit TUnit) TUnit)) ->
-  ctx:( (unit -> IST unit (fun _ -> True) (fun h0 _ h1 -> modifies_only_shared h0 h1)) -> 
-              IST unit (fun _ -> True) (fun h0 _ h1 -> modifies_only_shared h0 h1)) ->
-  IST unit 
-    (requires (fun h0 ->
-      h0 `contains` rp /\ h0 `contains` rs /\ h0 `contains` (sel h0 rs) /\
-      ~(shareS.is_shared rp h0) /\
-      shareS.is_shared rs h0 /\ shareS.is_shared (sel h0 rs) h0))
-    (ensures (fun h0 _ h1 -> sel h0 rp == sel h1 rp)) // the content of rp should stay the same before/ after calling the context
-
-// TODO: the callback of the program should be able to modify rp
-let progr_passing_callback_test rp rs f =
-  let h0 = get () in
-  let secret: ref int = alloc 0 in
-  let h1 = get () in
-  assume (next_addr h0 < next_addr h1); (** comes from alloc *)
-  shareS.share secret;
-  witness (contains_pred secret);
-  witness (shareS.is_shared secret);
-  let cb : (unit -> IST unit (fun _ -> True) (fun h0 _ h1 -> modifies_only_shared h0 h1)) = (fun _ -> 
-    let h0 = get () in
-    recall (contains_pred secret);
-    recall (shareS.is_shared secret);
-    secret := !secret + 1;
-    let h1 = get () in
-    assume (next_addr h0 <= next_addr h1);
-    ()) in
-  f cb
-
-val progr_getting_callback_test: 
-  rp: ref int -> 
-  rs: ref (ref int) ->
-  ctx:( unit -> 
-    IST ((unit -> IST unit (fun _ -> True) (fun h0 _ h1 -> modifies_only_shared h0 h1)))
-      (fun _ -> True)
-      (fun h0 _ h1 -> modifies_only_shared h0 h1)) ->
- // ctx:(elab_typ (TArr TUnit (TArr TUnit TUnit))) ->
-  IST unit 
-    (requires (fun h0 ->
-      h0 `contains` rp /\ h0 `contains` rs /\ h0 `contains` (sel h0 rs) /\
-      ~(shareS.is_shared rp h0) /\
-      shareS.is_shared rs h0 /\ shareS.is_shared (sel h0 rs) h0))
-    (ensures (fun h0 _ h1 -> sel h0 rp == sel h1 rp))
-
-let progr_getting_callback_test rp rs f =
-  let cb = f () in
-  cb ();
-  ()
-**)
+let lemma_same_addr_same_sharing_status = (fun ra rb h -> ())
